venom/passes/cfg_normalization/proofs/prevBbIndepScript.sml
@@ -433,7 +433,20 @@ Proof
   >- prev_bb_opcode_tac (* ASSIGN *)
   >- prev_bb_opcode_tac (* NOP *)
   >- prev_bb_opcode_tac (* ALLOCA *)
+  >- prev_bb_opcode_tac (* DALLOCA *)
+  >- prev_bb_opcode_tac (* DRET *)
+  >- prev_bb_opcode_tac (* GETFMP *)
+  >- prev_bb_opcode_tac (* SETFMP *)
+  >- prev_bb_opcode_tac (* RETFMP *)
+  >- prev_bb_opcode_tac (* INITIAL_FMP *)
+  >- (strip_tac >> gvs[] >>
+      ASM_REWRITE_TAC[step_inst_base_def] >>
+      simp[eval_op_prev_bb, exec_result_map_prev_bb_def] >>
+      BasicProvers.EVERY_CASE_TAC >>
+      simp[update_var_def, exec_result_map_prev_bb_def]) (* BUMP *)
   >- prev_bb_opcode_tac (* INVOKE *)
+  >- prev_bb_opcode_tac (* FMP_PARAM *)
+  >- prev_bb_opcode_tac (* RETPC_PARAM *)
   >- prev_bb_opcode_tac (* CALLER *)
   >- prev_bb_opcode_tac (* CALLVALUE *)
   >- prev_bb_opcode_tac (* CALLDATALOAD *)
