venom/passes/make_ssa/proofs/ssaSimDefsScript.sml
@@ -38,6 +38,10 @@ Theorem execution_equiv_UNIV:
     s1.vs_labels = s2.vs_labels /\
     s1.vs_code = s2.vs_code /\
     s1.vs_params = s2.vs_params /\
+    s1.vs_fmp = s2.vs_fmp /\
+    s1.vs_call_entry_fmp = s2.vs_call_entry_fmp /\
+    s1.vs_initial_fmp = s2.vs_initial_fmp /\
+    s1.vs_return_pc_token = s2.vs_return_pc_token /\
     s1.vs_prev_hashes = s2.vs_prev_hashes /\
     s1.vs_allocas = s2.vs_allocas /\
     s1.vs_alloca_next = s2.vs_alloca_next
@@ -74,6 +78,10 @@ Theorem step_inst_base_var_only_preserves_non_var:
     s'.vs_labels = s.vs_labels /\
     s'.vs_code = s.vs_code /\
     s'.vs_params = s.vs_params /\
+    s'.vs_fmp = s.vs_fmp /\
+    s'.vs_call_entry_fmp = s.vs_call_entry_fmp /\
+    s'.vs_initial_fmp = s.vs_initial_fmp /\
+    s'.vs_return_pc_token = s.vs_return_pc_token /\
     s'.vs_prev_hashes = s.vs_prev_hashes /\
     s'.vs_allocas = s.vs_allocas /\
     s'.vs_alloca_next = s.vs_alloca_next /\
@@ -111,6 +119,10 @@ Definition ssa_sim_def:
     s1.vs_labels = s2.vs_labels /\
     s1.vs_code = s2.vs_code /\
     s1.vs_params = s2.vs_params /\
+    s1.vs_fmp = s2.vs_fmp /\
+    s1.vs_call_entry_fmp = s2.vs_call_entry_fmp /\
+    s1.vs_initial_fmp = s2.vs_initial_fmp /\
+    s1.vs_return_pc_token = s2.vs_return_pc_token /\
     s1.vs_prev_hashes = s2.vs_prev_hashes /\
     s1.vs_allocas = s2.vs_allocas /\
     s1.vs_alloca_next = s2.vs_alloca_next /\
@@ -447,6 +459,10 @@ Theorem ssa_sim_non_var_update:
     s1'.vs_labels = s2'.vs_labels /\
     s1'.vs_code = s2'.vs_code /\
     s1'.vs_params = s2'.vs_params /\
+    s1'.vs_fmp = s2'.vs_fmp /\
+    s1'.vs_call_entry_fmp = s2'.vs_call_entry_fmp /\
+    s1'.vs_initial_fmp = s2'.vs_initial_fmp /\
+    s1'.vs_return_pc_token = s2'.vs_return_pc_token /\
     s1'.vs_prev_hashes = s2'.vs_prev_hashes /\
     s1'.vs_allocas = s2'.vs_allocas /\
     s1'.vs_alloca_next = s2'.vs_alloca_next /\
